% Notes and exercises from Set Theory by Jech
% By John Peloquin
\documentclass[letterpaper,12pt]{article}
\usepackage{amsmath,amssymb,amsthm,enumitem,fourier}

\newcommand{\N}{\boldsymbol{N}}
\renewcommand{\P}{P}
\newcommand{\Ord}{\mathit{Ord}}

\newcommand{\union}{\cup}
\newcommand{\bigunion}{\bigcup}
\newcommand{\sect}{\cap}
\newcommand{\bigsect}{\bigcap}
\newcommand{\after}{\circ}
\newcommand{\mult}{\cdot}

\newcommand{\suc}[1]{#1\union\{#1\}}
\newcommand{\preimage}[1]{#1_{-1}}
\newcommand{\card}[1]{|#1|}
\newcommand{\seq}[1]{\langle#1\rangle}

% Theorems
\theoremstyle{definition}
\newtheorem*{exer}{Exercise}

\theoremstyle{remark}
\newtheorem*{rmk}{Remark}

% Meta
\title{Notes and exercises from \textit{Set Theory}}
\author{John Peloquin}
\date{}

\begin{document}
\maketitle

\section*{Introduction}
This document contains notes and exercises from~\cite{jech}.

\section*{Chapter~1}
\begin{exer}[1.2]
There is no set~\(X\) such that \(\P(X)\subset X\).
\end{exer}
\begin{proof}
By the axiom of regularity~(1.8), \(X\)~is \(\in\)-minimal in~\(\{X\}\), so \(X\not\in X\) and hence \(\P(X)\not\subset X\).
\end{proof}

\begin{exer}[1.3]
If \(X\)~is inductive, then the set \(\{\,x\in X\mid x\subset X\,\}\) is inductive. Hence \(\N\)~is transitive and for each \(n\in\N\), \(n=\{\,m\in\N\mid m<n\,\}\).
\end{exer}
\begin{proof}
Let \(S=\{\,x\in X\mid x\subset X\,\}\). By inductivity of~\(X\), \(\emptyset\in S\), and if \(x\in S\), then \(\suc{x}\in S\), so \(S\)~is inductive. Taking \(X=\N\), it follows that \(S=\N\) since \(\N\)~is the smallest inductive set. Hence \(n\in\N\) implies \(n\subset\N\), so \(\N\)~is transitive and \(n=\{\,m\in\N\mid m<n\,\}\).
\end{proof}
\begin{rmk}
We proved transitivity of~\(\N\) ``by induction'' on~\(\N\): \(0\subset\N\) and if \(n\subset\N\) then \(n+1\subset\N\), so \(n\subset\N\) for all \(n\in\N\). The following exercises are similar.
\end{rmk}

\begin{exer}[1.4]
If \(X\)~is inductive, then the set \(\{\,x\in X\mid x\text{ is transitive}\,\}\) is inductive. Hence every \(n\in\N\) is transitive.
\end{exer}
\begin{proof}
The class~\(C\) of transitive sets is inductive. Indeed, \(\emptyset\)~is transitive, and if \(x\)~is transitive then \(\suc{x}\)~is transitive since \(y\in\suc{x}\) implies \(y\subset x\subset\suc{x}\). It follows that \(\{\,x\in X\mid x\text{ is transitive}\,\}=X\sect C\) is inductive since the intersection of two inductive classes is inductive. Taking \(X=\N\), it follows as above that every \(n\in\N\) is transitive.
\end{proof}

\begin{exer}[1.5]
If \(X\)~is inductive, then the set \(\{\,x\in X\mid x\text{ is transitive and }x\not\in x\,\}\) is inductive. Hence \(n\not\in n\) and \(n\ne n+1\) for all \(n\in\N\).
\end{exer}
\begin{proof}
The class \(C=\{\,x\mid x\text{ is transitive and }x\not\in x\,\}\) is inductive. Indeed, \(\emptyset\in C\). If \(x\in C\), then \(\suc{x}\)~is transitive (by inductivity of the class of transitive sets). Also \(\suc{x}\not\in x\), lest \(\suc{x}\subset x\) by transitivity of~\(x\) and hence \(x\in x\)---contradicting \(x\not\in x\). Similarly \(\suc{x}\not=x\). Therefore \(\suc{x}\not\in\suc{x}\). So \(\suc{x}\in C\), and \(C\)~is inductive. It follows as above that \(X\sect C\)~is inductive, and taking \(X=\N\) that \(n\not\in n\) and hence \(n\ne n+1\) for all \(n\in\N\).
\end{proof}

\begin{rmk}
In order to prove that \(n\not\in n\) for all \(n\in\N\) by induction on~\(\N\), we ``loaded the induction hypothesis'' with transitivity.
\end{rmk}

\begin{exer}[1.6]
If \(X\)~is inductive, then the set \(\{\,x\in X\mid x\text{ is transitive and regular}\,\}\) is inductive, where a set \(x\)~is called \emph{regular} if every nonempty subset of~\(x\) has an \(\in\)-minimal element.
\end{exer}
\begin{proof}
The class \(C=\{\,x\mid x\text{ is transitive and regular}\,\}\) is inductive. Indeed, \(\emptyset\in C\). If \(x\in C\), then \(\suc{x}\)~is transitive. If \(y\subset\suc{x}\) is nonempty, let \(z=y-\{x\}\subset x\). If \(z=\emptyset\), then \(y=\{x\}\), and \(x\)~is \(\in\)-minimal in~\(y\) by regularity of~\(x\). If \(z\ne\emptyset\) and \(t\)~is \(\in\)-minimal in~\(z\), then \(x\not\in t\) by transitivity and regularity of~\(x\), so \(t\)~is \(\in\)-minimal in~\(y\). Therefore \(\suc{x}\)~is regular. So \(\suc{x}\in C\), and \(C\)~is inductive. It follows as above that \(X\sect C\)~is inductive.
\end{proof}

\begin{rmk}
Taking \(X=\N\) it follows as above that every \(n\in\N\) is regular.
\end{rmk}

\begin{exer}[1.7]
Every nonempty \(X\subset\N\) has an \(\in\)-minimal element.
\end{exer}
\begin{proof}
Choose \(n\in X\). If \(n\)~is not \(\in\)-minimal in~\(X\), then \(n\sect X\)~is a nonempty subset of~\(n\), which has an \(\in\)-minimal element~\(m\) (Exercise~1.6). By transitivity of~\(n\) (Exercise~1.4), \(m\)~is \(\in\)-minimal in~\(X\).
\end{proof}

\begin{exer}[1.8]
If \(X\)~is inductive, then the set \(\{\,x\in X\mid x=\emptyset\text{ or }\exists y(x=\suc{y})\,\}\) is inductive. Hence for all \(n\in\N\), \(n=0\) or \(n=m+1\) for some \(m\in\N\).
\end{exer}
\begin{proof}
The class \(C=\{\,x\mid x=\emptyset\text{ or }\exists y(x=\suc{y})\,\}\) is obviously inductive, so \(X\sect C\)~is inductive. Taking \(X=\N\), the rest follows, with \(m\in\N\) by transitivity of~\(\N\) (Exercise~1.3).
\end{proof}

\begin{exer}[1.9]
Let \(A\subset\N\) be such that \(0\in A\), and if \(n\in A\) then \(n+1\in A\). Then \(A=\N\).
\end{exer}
\begin{proof}
\(A\)~is inductive, so \(A=\N\) since \(\N\)~is the smallest inductive set.

Alternately, if \(A\ne\N\), let \(m\)~be \(\in\)-minimal in \(\N-A\) (Exercise~1.7). Then \(m\ne0\), and \(m\ne n+1\) for any \(n\in\N\), which is impossible (Exercise~1.8).
\end{proof}

\begin{exer}[1.10]
Each \(n\in\N\) is T-finite.
\end{exer}
\begin{proof}
By induction on~\(\N\). First, \(n=0\)~is T-finite since \(\P(\emptyset)=\{\emptyset\}\) and \(\emptyset\)~is \(\subset\)-maximal in~\(\{\emptyset\}\). If \(n\)~is T-finite, suppose \(X\subset\P(\suc{n})\) is nonempty. Let
\[X'=\{\,u-\{n\}\mid u\in X\,\}\]
Then \(X'\subset\P(n)\) is nonempty and has a \(\subset\)-maximal element \(u-\{n\}\) for some \(u\in X\) by T-finiteness of~\(n\), where we may assume \(n\in u\) if \(u\union\{n\}\in X\). We claim \(u\)~is \(\subset\)-maximal in~\(X\). Indeed, if \(v\in X\) and \(u\subset v\), then \(u-\{n\}\subset v-\{n\}\), so \(u-\{n\}=v-\{n\}\) by \(\subset\)-maximality of~\(u-\{n\}\) in~\(X'\), so \(u=v\) by the assumption about~\(u\). Therefore \(n+1\)~is T-finite.
\end{proof}

\begin{exer}[1.11]
\(\N\)~is T-infinite. In fact, \(\N\subset\P(\N)\) has no \(\subset\)-maximal element.
\end{exer}
\begin{proof}
We know \(\N\subset\P(\N)\) by transitivity of~\(\N\) (Exercise~1.3), and for all \(n\in\N\) we have \(n\subset n+1\in\N\) but \(n\ne n+1\) (Exercise~1.5).
\end{proof}

\begin{rmk}
If \(A\)~is T-finite and \(\pi:A\to B\) is surjective (onto), then \(B\)~is T-finite.
\end{rmk}
\begin{proof}
By pullback. If \(X\subset\P(B)\) is nonempty, let
\[\preimage{X}=\preimage{\pi}(X)=\{\,\preimage{u}=\preimage{\pi}(u)\mid u\in X\,\}\]
Then \(\preimage{X}\subset\P(A)\) is nonempty and has a \(\subset\)-maximal element \(\preimage{u}\) for some \(u\in X\) by T-finiteness of~\(A\). We claim \(u\)~is \(\subset\)-maximal in~\(X\). Indeed, if \(v\in X\) and \(u\subset v\), then \(\preimage{u}\subset\preimage{v}\), so \(\preimage{u}=\preimage{v}\) by \(\subset\)-maximality of~\(\preimage{u}\) in~\(\preimage{X}\), so \(u=v\) by surjectivity of~\(\pi\). Therefore \(B\)~is T-finite.
\end{proof}

\begin{exer}[1.12]
Every finite set is T-finite.
\end{exer}
\begin{proof}
By definition, every finite set is the image of a T-finite natural number (Exercise~1.10), so is T-finite by the previous remark.

Alternately, if \(S\)~is T-infinite, choose \(X\subset\P(S)\) nonempty with no \(\subset\)-maximal element. By induction on~\(\N\), for each \(n\in\N\) there is a properly ascending chain \(u_0\subset\cdots\subset u_n\subset S\) of length~\(n+1\) in~\(X\), and hence an injection \(n\to S\) sending \(m\in n\) into \(u_{m+1}-u_m\). If \(S\)~had \(k\)~elements for some \(k\in\N\), there would then be an injection \(k+1\to k\), which is impossible by an easy induction on~\(k\). Therefore \(S\)~is infinite.
\end{proof}

\begin{exer}[1.13]
Every infinite set is T-infinite.
\end{exer}
\begin{proof}
If \(S\)~is infinite, let \(X\)~be the set of finite subsets of~\(S\). Clearly \(X\)~is nonempty since \(\emptyset\in X\). Also \(X\)~has no \(\subset\)-maximal element. Indeed, if \(u\in X\) then there is \(s\in S-u\) since \(S\)~is infinite, and \(u\union\{s\}\)~is finite (if \(u\)~has \(k\)~elements, then \(u\union\{s\}\)~has \(k+1\) elements), so \(u\subset u\union\{s\}\in X\) where the inclusion is proper. Therefore \(S\)~is T-infinite.
\end{proof}

\begin{rmk}
The previous two exercises show that (Cantor) finiteness is equivalent to Tarski finiteness in~ZF.
\end{rmk}

\section*{Chapter~2}
\begin{rmk}
In~(2.1), \(<\)~is actually a \emph{well-ordering} on~\(\Ord\). Indeed, if \(C\subset\Ord\) is a nonempty class of ordinals and \(\alpha\in C\) is not \(\in\)-minimal in~\(C\), then \(\alpha\sect C\)~is a nonempty subset of~\(\alpha\) which has an \(\in\)-minimal element~\(\beta\). By transitivity of~\(\alpha\), \(\beta\)~is \(\in\)-minimal in~\(C\).

This observation provides an alternative proof that \(\Ord\)~is a proper class: if \(\Ord\)~were a set, then because it is transitive and strictly well-ordered by~\(\in\), it would be an ordinal, and hence \(\Ord\in\Ord\)---contradicting strictness.
\end{rmk}

\begin{exer}[2.2]
\(\alpha\)~is a limit ordinal if and only if \(\beta<\alpha\) implies \(\beta+1<\alpha\) for all~\(\beta\).
\end{exer}
\begin{proof}
If \(\alpha\)~is a limit ordinal and \(\beta<\alpha\), then \(\beta+1\le\alpha\) (2.5) and \(\beta+1\ne\alpha\), so \(\beta+1<\alpha\). If \(\alpha\)~is not a limit ordinal, then \(\beta+1=\alpha\) for some~\(\beta<\alpha\).
\end{proof}
\begin{rmk}
It follows that \(\alpha\)~is a nonzero limit ordinal if and only if it is inductive.
\end{rmk}

\begin{exer}[2.3]
If \(X\)~is inductive, then \(X\sect\Ord\)~is inductive. \(\N\)~is the least nonzero limit ordinal, where \(\N=\bigsect\{\,X\mid X\text{ inductive}\,\}\).
\end{exer}
\begin{proof}
Clearly \(\Ord\)~is inductive, so \(X\sect\Ord\)~is inductive since the intersection of two inductive classes is inductive. Taking \(X=\N\), it follows that \(\N\subset\Ord\), and since \(\N\)~is also transitive, \(\N\)~is an ordinal. By the previous remark, \(\N\)~is the least nonzero limit ordinal.
\end{proof}

\begin{exer}[2.4]
(Without the axiom of infinity.) Let \(\omega\)~be the least nonzero limit ordinal, if it exists, or~\(\Ord\) otherwise. The following are equivalent:
\begin{enumerate}[itemsep=0pt]
\item[(i)] There exists an inductive set.
\item[(ii)] There exists an infinite\footnote{In this exercise, a set is \emph{finite} if it is in bijective correspondence with some \(n\in\omega\) and \emph{infinite} otherwise, even if \(\omega=\Ord\).} set.
\item[(iii)] \(\omega\)~is a set.
\end{enumerate}
\end{exer}
\begin{proof}
(i) \(\iff\) (iii): The smallest inductive set is the least nonzero limit ordinal (Exercise~2.3).

(iii) \(\implies\) (ii): \(\omega\)~is infinite (Exercises 1.11--2).

(ii) \(\implies\) (i): For any finite set~\(A\), let \(\card{A}\)~denote the least \(n\in\omega\) in bijective correspondence with~\(A\) (the ``number of elements'' in~\(A\)). If \(X\)~is infinite, let
\[S=\{\,\card{A}\mid A\subset X\text{ finite}\,\}\]
Note \(S\)~is a set by replacement, and \(S\)~is inductive. Indeed, \(0\in S\) since \(\emptyset\subset X\) and \(\card{\emptyset}=0\). If \(n\in S\) and \(A\subset X\) with \(\card{A}=n\), then there must exist \(x\in X-A\) since \(X\)~is infinite, and \(\card{A\union\{x\}}=n+1\in S\).
\end{proof}
\begin{rmk}
This exercise shows that (i)--(iii) are equivalent forms of the axiom of infinity in~ZF.
\end{rmk}

\begin{exer}[2.5]
If \(W\)~is a well-ordered set, then there is no sequence \(\seq{\,a_n\mid n\in\N\,}\) in~\(W\) such that \(a_0>a_1>\cdots\)\ .
\end{exer}
\begin{proof}
If there were such a sequence, then \(\{\,a_n\mid n\in\N\,\}\) would be a nonempty subset of~\(W\) with no least element, contradicting well-ordering.
\end{proof}

\begin{exer}[2.6]
There are arbitrarily large limit ordinals.
\end{exer}
\begin{proof}
Given~\(\alpha\), let \(\beta=\alpha+\omega\). Clearly \(\beta>\alpha\). If \(\gamma<\beta\), then either \(\gamma<\alpha\), in which case \(\gamma+1<\alpha+1<\beta\), or \(\gamma\ge\alpha\), in which case \(\gamma=\alpha+n\) for some \(n\in\omega\) (Lemma~2.25), so \(\gamma+1=\alpha+n+1<\beta\). Thus \(\beta\)~is a limit ordinal (Exercise~2.2).
\end{proof}

\begin{rmk}[Chain rule]
If \(f,g:\Ord\to\Ord\) are nondecreasing and continuous, then so is~\(f\after g\). If \(f\)~and~\(g\) are normal, then so is~\(f\after g\).
\end{rmk}
\begin{proof}
If \(\alpha<\beta\), then \(g(\alpha)\le g(\beta)\), so \(f(g(\alpha))\le f(g(\beta))\). Let \(\alpha\)~be a nonzero limit ordinal. Clearly \(f(g(\alpha))\ge\lim_{\xi\to\alpha}f(g(\xi))\). If \(g(\alpha)=g(\xi')\) for some \(\xi'<\alpha\), then \(f(g(\alpha))=f(g(\xi'))\le\lim_{\xi\to\alpha}f(g(\xi))\). Otherwise, \(g(\alpha)\)~is a limit ordinal. Indeed, \(g(\alpha)=\lim_{\xi\to\alpha}g(\xi)\) by continuity of~\(g\), so if \(\beta<g(\alpha)\), then \(\beta<g(\xi)\) for some \(\xi<\alpha\), and hence \(\beta+1\le g(\xi)<g(\alpha)\). But then \(f(g(\alpha))=\lim_{\zeta\to g(\alpha)}f(\zeta)\) by continuity of~\(f\). If \(\zeta<g(\alpha)\), then \(\zeta<g(\xi)\) for some \(\xi<\alpha\), so \(f(\zeta)\le f(g(\xi))\), and hence \(\lim_{\zeta\to g(\alpha)}f(\zeta)\le\lim_{\xi\to\alpha}f(g(\xi))\). Therefore again \(f(g(\alpha))=\lim_{\xi\to\alpha}f(g(\xi))\) and \(f\after g\)~is continuous.

If \(f\)~and~\(g\) are also increasing, then \(f\after g\)~is increasing and hence normal.
\end{proof}

\begin{exer}[2.7]
Every normal sequence \(\seq{\,\gamma_{\alpha}\mid\alpha\in\Ord\,}\) has arbitrarily large fixed points (that is, \(\beta\)~such that \(\gamma_{\beta}=\beta\)).
\end{exer}
\begin{proof}
Given~\(\alpha\), let \(\beta_0=\gamma_{\alpha}\) and \(\beta_{n+1}=\gamma_{\beta_n}\) for all \(n\in\omega\). Note \(\beta_{n+1}\ge\beta_n\ge\alpha\) for all \(n\in\omega\) since \(\gamma\)~is increasing (Lemma~2.4). Let \(\beta=\lim_{n\to\omega}\beta_n\). Then
\[\gamma_{\beta}=\lim_{n\to\omega}\gamma_{\beta_n}=\lim_{n\to\omega}\beta_{n+1}=\beta\]
by the chain rule above (taking \(\beta_{\alpha}=\beta\) for all \(\alpha\ge\omega\)).
\end{proof}

\begin{exer}[2.8]
For all \(\alpha,\beta,\gamma\):
\begin{enumerate}[itemsep=0pt]
\item[(i)] \(\alpha\mult(\beta+\gamma)=\alpha\mult\beta+\alpha\mult\gamma\)
\item[(ii)] \(\alpha^{\beta+\gamma}=\alpha^{\beta}\mult\alpha^{\gamma}\)
\item[(iii)] \((\alpha^{\beta})^{\gamma}=\alpha^{\beta\mult\gamma}\)
\end{enumerate}
\end{exer}
\begin{proof}
By induction on~\(\gamma\).
\begin{enumerate}[itemsep=0pt]
\item[(i)] If \(\gamma=0\),
\[\alpha\mult(\beta+\gamma)=\alpha\mult(\beta+0)=\alpha\mult\beta=\alpha\mult\beta+0=\alpha\mult\beta+\alpha\mult 0=\alpha\mult\beta+\alpha\mult\gamma\]
If the result holds for~\(\gamma\), then
\begin{align*}
\alpha\mult(\beta+(\gamma+1))&=\alpha\mult((\beta+\gamma)+1)&&\text{by associativity of~\(+\)}\\
	&=\alpha\mult(\beta+\gamma)+\alpha&&\text{by definition of~\(\mult\)}\\
	&=(\alpha\mult\beta+\alpha\mult\gamma)+\alpha&&\text{by hypothesis}\\
	&=\alpha\mult\beta+(\alpha\mult\gamma+\alpha)&&\text{by associativity of~\(+\)}\\
	&=\alpha\mult\beta+\alpha\mult(\gamma+1)&&\text{by definition of~\(\mult\)}
\end{align*}
so the result holds for~\(\gamma+1\). If \(\gamma\)~is a nonzero limit ordinal and the result holds for all \(\xi<\gamma\), then
\begin{align*}
\alpha\mult(\beta+\gamma)&=\lim_{\xi\to\gamma}\alpha\mult(\beta+\xi)&&\text{by continuity of }\xi\mapsto\alpha\mult(\beta+\xi)\\
	&=\lim_{\xi\to\gamma}(\alpha\mult\beta+\alpha\mult\xi)&&\text{by hypothesis}\\
	&=\alpha\mult\beta+\alpha\mult\gamma&&\text{by continuity of }\xi\mapsto\alpha\mult\beta+\alpha\mult\xi
\end{align*}
so the result holds for~\(\gamma\). Note that continuity of the composite mappings involved follows from continuity of addition and multiplication and the chain rule above.
\item[(ii)] Similar.
\item[(iii)] Similar, using (i)~and~(ii) in the successor step.\qedhere
\end{enumerate}
\end{proof}

\begin{exer}[2.9]\
\begin{enumerate}[itemsep=0pt]
\item[(i)] \((\omega+1)\mult 2=\omega+1+\omega+1=\omega+\omega+1=\omega\mult 2+1<\omega\mult 2+2=\omega\mult 2+1\mult 2\)
\item[(ii)] \((\omega\mult 2)^2=\omega\mult 2\mult\omega\mult 2=\omega\mult\omega\mult 2=\omega^2\mult 2<\omega^2\mult 4=\omega^2\mult 2^2\)
\end{enumerate}
\end{exer}
\begin{rmk}
This result shows that \((\alpha+\beta)\mult\gamma\) does not in general equal \(\alpha\mult\gamma+\beta\mult\gamma\), and \((\alpha\mult\beta)^{\gamma}\) does not in general equal \(\alpha^{\gamma}\mult\beta^{\gamma}\).
\end{rmk}

\begin{exer}[2.10]
If \(\alpha<\beta\), then \(\alpha+\gamma\le\beta+\gamma\), \(\alpha\mult\gamma\le\beta\mult\gamma\), and \(\alpha^{\gamma}\le\beta^{\gamma}\) for all~\(\gamma\).
\end{exer}
\begin{proof}
By induction on~\(\gamma\).
\end{proof}

\begin{exer}[2.11]
\(2<3\) but
\begin{enumerate}[itemsep=0pt]
\item[(i)] \(2+\omega=\omega=3+\omega\)
\item[(ii)] \(2\mult\omega=\omega=3\mult\omega\)
\item[(iii)] \(2^{\omega}=\omega=3^{\omega}\)
\end{enumerate}
\end{exer}

\begin{exer}[2.12]
Let \(\epsilon_0=\lim_{n\to\omega}\alpha_n\) where \(\alpha_0=\omega\) and \(\alpha_{n+1}=\omega^{\alpha_n}\). Then \(\epsilon_0\)~is the least ordinal~\(\epsilon\) such that \(\omega^{\epsilon}=\epsilon\).
\end{exer}
\begin{proof}
By continuity of exponentiation and the chain rule above (taking \(\alpha_{\beta}=\epsilon_0\) for all \(\beta\ge\omega\)),
\[\omega^{\epsilon_0}=\lim_{n\to\omega}\omega^{\alpha_n}=\lim_{n\to\omega}\alpha_{n+1}=\epsilon_0\]
If \(\omega^{\epsilon}=\epsilon\), we prove by induction that \(\alpha_n\le\epsilon\) for all \(n\in\omega\), from which it follows that \(\epsilon_0\le\epsilon\). Indeed, since \(\omega^0=1\ne0\), we have \(\epsilon\ne 0\) and hence \(\alpha_0=\omega\le\omega^{\epsilon}=\epsilon\). If \(\alpha_n\le\epsilon\), then \(\alpha_{n+1}=\omega^{\alpha_n}\le\omega^{\epsilon}=\epsilon\).
\end{proof}

\begin{exer}[2.13]
A limit ordinal \(\gamma>0\) is indecomposable if and only if \(\alpha+\gamma=\gamma\) for all \(\alpha<\gamma\) if and only if \(\gamma=\omega^{\alpha}\) for some~\(\alpha>0\).
\end{exer}
\begin{proof}
If \(\gamma=\alpha+\beta\) with \(\alpha,\beta<\gamma\), then \(\alpha+\gamma>\alpha+\beta=\gamma\). Conversely, if \(\alpha<\gamma\) and \(\alpha+\gamma>\gamma\), fix~\(\beta\) such that \(\alpha+\beta=\gamma\) (Lemma~2.25). If \(\beta\ge\gamma\), then \(\gamma=\alpha+\beta\ge\alpha+\gamma>\gamma\), which is impossible, so \(\beta<\gamma\).

The forward direction of the second equivalence follows from the Cantor normal form (Theorem~2.26). For the reverse direction, we prove by induction on \(\alpha>0\) that \(\omega^{\alpha}\)~is indecomposable. The result holds for \(\alpha=1\) since \(n+\omega=\omega\) for all \(n\in\omega\). If \(\omega^{\alpha}\)~is indecomposable and \(\beta<\omega^{\alpha+1}=\omega^{\alpha}\mult\omega\), then \(\beta<\omega^{\alpha}\mult n\) for some \(n\in\omega\), so (Exercises 2.10 and 2.8)
\[\beta+\omega^{\alpha+1}\le\omega^{\alpha}\mult n+\omega^{\alpha}\mult\omega=\omega^{\alpha}\mult(n+\omega)=\omega^{\alpha}\mult\omega=\omega^{\alpha+1}\]
and hence \(\omega^{\alpha+1}\)~is indecomposable. Finally if \(\alpha>0\)~is a limit ordinal, \(\omega^{\xi}\)~is indecomposable for all \(\xi<\alpha\), and \(\beta<\omega^{\alpha}\), then by continuity
\[\beta+\omega^{\alpha}=\lim_{\xi\to\alpha}(\beta+\omega^{\xi})=\lim_{\xi\to\alpha}\omega^{\xi}=\omega^{\alpha}\]
and hence \(\omega^{\alpha}\)~is indecomposable.
\end{proof}

% References
\begin{thebibliography}{0}
\bibitem{jech} Jech, Thomas. \textit{Set Theory}, 3rd~ed. Springer, 2002.
\end{thebibliography}
\end{document}
